Infra/Relations2.v
@@ -1,0 +1,25 @@
+Require Import Arith Coq.Lists.List Setoid Coq.Lists.SetoidList Util.
+Require Export Infra.Option EqDec AutoIndTac Tactics.
+
+Set Implicit Arguments.
+
+Definition functional2 :=
+fun (X Y : Type) (R : X -> Y -> X -> Prop)
+=> forall x (y:Y) x1 x2, R x y x1 -> R x y x2 -> x1 = x2.
+
+Definition reducible2 :=
+fun (X Y : Type) (R : X->Y->X->Prop) (x : X) => exists y x', R x y x'.
+
+Definition normal2 :=
+fun (X Y : Type) (R : X->Y->X->Prop) (x : X) => ~ reducible2 R x.
+
+Definition reddec :=
+fun (X Y : Type) (R : X->Y->X->Prop) => forall x : X, reducible2 R x \/ normal2 R x.
+
+
+
+(*
+*** Local Variables: ***
+*** coq-load-path: (("../" "Lvc")) ***
+*** End: ***
+*)
